Iris/Iris/Std/List.lean
@@ -60,19 +60,19 @@ theorem fresh [InfiniteType A] (X : List A) : ∃ a : A, a ∉ X := by
   omega
 
 @[expose, match_pattern]
-def List.Forall₂.append : ∀ {l₁ l₁' l₂ l₂'}, List.Forall₂ R l₁ l₂ → List.Forall₂ R l₁' l₂' → List.Forall₂ R (l₁ ++ l₁') (l₂ ++ l₂')
+def Forall₂.append : ∀ {l₁ l₁' l₂ l₂'}, List.Forall₂ R l₁ l₂ → List.Forall₂ R l₁' l₂' → List.Forall₂ R (l₁ ++ l₁') (l₂ ++ l₂')
   | _, _, _, _, .nil, h => h
   | _, _, _, _, .cons step rest, h => .cons step (append rest h)
 
 @[grind →]
-theorem List.exists_of_forall₂_cons : ∀ {l₁ l₂}{x},
+theorem exists_of_forall₂_cons : ∀ {l₁ l₂}{x},
     List.Forall₂ R (x :: l₁) l₂ → ∃ y l₂', l₂ = y :: l₂' ∧ R x y ∧ List.Forall₂ R l₁ l₂' := by
   intro l₁ l₂ x h
   cases h with
   | cons y l₂' => grind only
 
 @[grind →]
-theorem List.exists_of_forall₂_append : ∀ {l₁ l₁' l},
+theorem exists_of_forall₂_append : ∀ {l₁ l₁' l},
     List.Forall₂ R (l₁ ++ l₁') l → ∃ l₂ l₂', l = l₂ ++ l₂' ∧ List.Forall₂ R l₁ l₂ ∧ List.Forall₂ R l₁' l₂' ∧ l₁.length = l₂.length := by
   intro l₁ l₁' l h
   induction l₁ generalizing l with
@@ -87,5 +87,23 @@ theorem List.exists_of_forall₂_append : ∀ {l₁ l₁' l},
     -- exists (y :: l₂), l₂'
     -- refine ⟨h ▸ rfl, List.Forall₂.cons x_y Rleft, Rright, ?_⟩
     -- simp only [List.length_cons, hlen]
+
+@[grind =]
+theorem getElem?_some_iff_append
+{a : α} {i : Nat} {l : List α} : l[i]? = some a ↔ ∃ s t : List α, l = s ++ a :: t ∧ s.length = i := by
+  constructor
+  · intros h
+    induction i generalizing l with
+    | zero =>
+      rcases l with _ | ⟨hd, tl⟩
+      · simp at h
+      · simpa using h
+    | succ i IH =>
+      rcases l with _ | ⟨hd, tl⟩
+      · simp at h
+      simp at h
+      grind only [=_ List.cons_append, = List.length_cons]
+  · rintro ⟨ps, ss, rfl, h2⟩
+    grind only [= List.getElem?_append, = List.getElem?_cons]
 
 end Iris.Std.List
