Iris/Iris/Std/Relation.lean
@@ -1,6 +1,10 @@
 module
 
-@[expose] public section
+public import Iris.Std.FromMathlib
+
+open FromMathlib
+
+public section
 
 namespace Relation
 
@@ -10,3 +14,22 @@ inductive iterate {α : Type _} (R : α → α → Prop) : Nat → α → α →
 | tail (y: α) {n : Nat}{x z : α} : iterate R n x y → R y z → iterate R (n+1) x z
 
 attribute [simp] iterate.rfl iterate.tail
+
+theorem ReflTrans_iff_exists_iterate {α : Type _} {R : α → α → Prop} :
+    ∀ {x y},
+    Relation.ReflTransGen R x y ↔ ∃ n, Relation.iterate R n x y := by
+  intros x y
+  constructor
+  · intros rtcR
+    induction rtcR with
+    | refl =>
+      exists 0; constructor
+    | tail rtcMid Rlast IH =>
+      obtain ⟨n, h⟩ := IH
+      exists (n+1)
+      apply Relation.iterate.tail _ h Rlast
+  · rintro ⟨n, itR⟩
+    induction itR with
+    | rfl => constructor
+    | tail z itMid Rlast IH =>
+      apply Relation.ReflTransGen.tail IH Rlast
